Update

theories/Logic/ClassicalFol.v
@@ -51,147 +51,11 @@ Section COMPLETENESS_OF_HilbertCalculus.
 
 Import FolHilbert.
 
-#[local] Existing Instance V.vec_isSetoid.
-
-Context {L : language} {enum_function_symbols : isEnumerable L.(function_symbols)} {enum_constant_symbols : isEnumerable L.(constant_symbols)} {enum_relation_symbols : isEnumerable L.(relation_symbols)}.
+Context {L : language} {function_symbols_countable : isCountable L.(function_symbols)} {constant_symbols_countable : isCountable L.(constant_symbols)} {relation_symbols_countable : isCountable L.(relation_symbols)}.
 
 Notation L' := (augmented_language L Henkin_constants).
 
-#[local]
-Instance augmented_language_isEnumerable : isEnumerable (frm L') :=
-  @frm_isEnumerable L' enum_function_symbols (@sum_isEnumerable L.(constant_symbols) Henkin_constants enum_constant_symbols nat_isEnumerable) enum_relation_symbols.
-
-Section MODEL_EXISTENCE.
-
-Variable X : ensemble (frm L).
-
-Let Delta : ensemble (frm L') :=
-  MaximallyConsistentSet (AddHenkin (E.image embed_frm X)).
-
-Let D : Type :=
-  trm L'.
-
-Definition interpret_equation (lhs : D) (rhs : D) : Prop :=
-  Delta ⊢ Eqn_frm lhs rhs.
-
-#[global]
-Instance interpret_equation_Equivalence
-  : Equivalence interpret_equation.
-Proof with eauto.
-  unfold interpret_equation. split.
-  - intros x. eapply proves_reflexivity...
-  - intros x y EQ. eapply proves_symmetry...
-  - intros x y z EQ EQ'. eapply proves_transitivity...
-Qed.
-
-Lemma pairwise_equal_intro n vs1 vs2
-  (EQ : forall i : Fin.t n, interpret_equation (vs1 !! i) (vs2 !! i))
-  : pairwise_equal Delta (vec_to_trms vs1) (vec_to_trms vs2).
-Proof.
-  revert vs2 EQ. induction vs1 as [ | n v1 vs1 IH].
-  - introVNil; simpl; i. econs.
-  - introVCons v2 vs2; simpl; i. econs.
-    + eapply EQ with (i := FZ).
-    + eapply IH. intros i. eapply EQ with (i := FS i).
-Qed.
-
-Lemma pairwise_equal_symmetry n (vs1 : Vector.t (trm L') n) (vs2 : Vector.t (trm L') n)
-  (EQUAL : pairwise_equal Delta (vec_to_trms vs1) (vec_to_trms vs2))
-  : pairwise_equal Delta (vec_to_trms vs2) (vec_to_trms vs1).
-Proof.
-  revert vs2 EQUAL. induction vs1 as [ | n v1 vs1 IH].
-  - introVNil; simpl; i. econs.
-  - introVCons v2 vs2; simpl; intros [EQ EQUAL]. econs.
-    + eapply proves_symmetry; trivial.
-    + eapply IH; trivial.
-Qed.
-
-#[local, program]
-Instance mkModel : isStructureOf L' :=
-  { domain_of_discourse := D
-  ; equation_interpret := {| eqProp := interpret_equation; eqProp_Equivalence := interpret_equation_Equivalence |}
-  ; function_interpret f vs := Fun_trm f (vec_to_trms vs)
-  ; constant_interpret c := Con_trm c
-  ; relation_interpret R vs := Delta ⊢ Rel_frm R (vec_to_trms vs)
-  }.
-Next Obligation.
-  econs. exact (Var_trm 0).
-Qed.
-Next Obligation.
-  red. eapply proves_eqn_fun. eapply pairwise_equal_intro; trivial.
-Qed.
-Next Obligation.
-  split; intros INFERS.
-  - eapply for_Imp_E. eapply proves_eqn_rel. 2: exact INFERS. eapply pairwise_equal_intro; trivial.
-  - eapply for_Imp_E. eapply proves_eqn_rel. 2: exact INFERS. eapply pairwise_equal_symmetry; eapply pairwise_equal_intro; trivial.
-Qed.
-
-Definition ivar_interpret : ivar -> domain_of_discourse :=
-  Var_trm.
-
-Lemma interpret_trm_MkModel_ivar_interpret (t : trm L')
-  : interpret_trm mkModel ivar_interpret t = t
-with interpret_trms_MkModel_ivar_interpret n (ts : trms L' n)
-  : vec_to_trms (interpret_trms mkModel ivar_interpret ts) = ts.
-Proof.
-  - trm_ind t; simpl.
-    + reflexivity.
-    + rewrite interpret_trm_unfold. simpl. f_equal. eapply interpret_trms_MkModel_ivar_interpret.
-    + reflexivity.
-  - trms_ind ts.
-    + reflexivity.
-    + rewrite interpret_trms_unfold. simpl. f_equal.
-      * eapply interpret_trm_MkModel_ivar_interpret.
-      * eapply IH.
-Qed.
-
-Theorem mkModel_isModel (p : frm L')
-  (CONSISTENT : X ⊬ Bot_frm)
-  : p \in Delta <-> interpret_frm mkModel ivar_interpret p.
-Proof with eauto with *.
-  exploit (@theorem_of_1_2_14 (frm L') (@formula_isSetoid L') LindenbaumBooleanAlgebra (Th (AddHenkin (E.image embed_frm X)))).
-  { eapply lemma1_of_1_3_8. }
-  intros [SUBSET' IS_FILTER' COMPLETE' EQUICONSISTENT']. fold (MaximallyConsistentSet (AddHenkin (E.image embed_frm X))) in SUBSET', IS_FILTER', COMPLETE', EQUICONSISTENT'.
-  fold Delta in SUBSET', IS_FILTER', COMPLETE', EQUICONSISTENT'.
-  pose proof (theorem_of_1_3_10 X) as [? ? ? ? ? ?]. fold Delta in SUBSET, EQUICONSISTENT, CLOSED_infers, META_DN, IMPLICATION_FAITHFUL, FORALL_FAITHFUL. unnw.
-  assert (CONSISTENT' : Delta ⊬ Bot_frm).
-  { intros INCONSISTENT.
-    assert (claim1 : ~ inconsistent' Delta).
-    { red in EQUICONSISTENT'. rewrite <- EQUICONSISTENT'. rewrite <- cl_eq_Th. rewrite <- inconsistent_okay. rewrite <- AddHenkin_equiconsistent.
-      - rewrite <- similar_equiconsistent with (Gamma := X).
-        + rewrite inconsistent_iff; trivial.
-        + rewrite <- embed_frms_spec. reflexivity.
-      - ii. rewrite E.in_image_iff in H. destruct H as [q [-> IN]]. eapply embed_frm_HC_free.
-    }
-    contradiction claim1. rewrite <- inconsistent_iff in INCONSISTENT.
-    rewrite inconsistent_okay in INCONSISTENT. eapply inconsistent_compatWith_isSubsetOf... eapply fact5_of_1_2_8...
-  }
-  rewrite CLOSED_infers. pattern p. revert p. eapply @frm_depth_lt_ind. intros [R ts | t1 t2 | p1 | p1 p2 | y p1]; simpl; i.
-  - rewrite interpret_trms_MkModel_ivar_interpret. reflexivity.
-  - do 2 rewrite interpret_trm_MkModel_ivar_interpret. reflexivity.
-  - rewrite <- IH with (p' := p1). 2: lia. split.
-    + intros INFERS1 INFERS2. contradiction CONSISTENT'.
-      eapply ContradictionI with (A := p1); trivial.
-    + intros NO. eapply NNPP. intros CONTRA. contradiction NO.
-      rewrite <- CLOSED_infers. eapply META_DN. intros INFERS. rewrite CLOSED_infers in INFERS. contradiction.
-  - rewrite <- IH with (p' := p1). 2: lia. rewrite <- IH with (p' := p2). 2: lia. split.
-    + intros INFERS1 INFERS2. eapply ImplicationE with (A := p1); trivial.
-    + intros INFERS. rewrite <- CLOSED_infers. eapply IMPLICATION_FAITHFUL. do 2 rewrite CLOSED_infers; trivial.
-  - unfold D. split.
-    + intros INFERS t. rename y into x. set (s := one_subst x t).
-      assert (IFF : interpret_frm mkModel ivar_interpret (subst_frm s p1) <-> interpret_frm mkModel (upd_env x t ivar_interpret) p1).
-      { rewrite <- substitution_lemma_frm. eapply interpret_frm_ext. ii. unfold compose, upd_env, s, one_subst, cons_subst, nil_subst.
-        destruct (eq_dec z x) as [EQ1 | NE1]; trivial. eapply interpret_trm_MkModel_ivar_interpret.
-      }
-      rewrite <- IFF. rewrite <- IH with (p' := subst_frm s p1). 2: rewrite subst_preserves_rank; lia.
-      unfold s. eapply for_All_E; trivial.
-    + intros INTERPRET. rewrite <- CLOSED_infers. eapply FORALL_FAITHFUL.
-      intros t. eapply CLOSED_infers. rewrite -> IH with (p' := subst_frm (one_subst y t) p1). 2: rewrite subst_preserves_rank; lia.
-      rewrite <- substitution_lemma_frm. eapply interpret_frm_ext with (env' := upd_env y (interpret_trm mkModel ivar_interpret t) ivar_interpret). ii. unfold compose, upd_env, one_subst, cons_subst, nil_subst.
-      destruct (eq_dec z y) as [EQ1 | NE1]; trivial. eapply INTERPRET.
-Qed.
-
-End MODEL_EXISTENCE.
+#[local] Existing Instance trmModel.
 
 #[local] Hint Resolve fact1_of_1_2_8 fact2_of_1_2_8 fact3_of_1_2_8 fact4_of_1_2_8 fact5_of_1_2_8 lemma1_of_1_2_11 : core.
 
@@ -203,16 +67,13 @@ Proof with eauto with *.
   set (Gamma := E.insert (Neg_frm b) X).
   assert (CONSISTENT : Gamma ⊬ Bot_frm).
   { intros INCONSISTENT. contradiction NO. eapply NegationE... }
-  exploit (@theorem_of_1_2_14 (frm L') (@formula_isSetoid L') LindenbaumBooleanAlgebra (Th (AddHenkin (E.image embed_frm Gamma)))).
-  { eapply lemma1_of_1_3_8. }
-  intros [SUBSET' IS_FILTER' COMPLETE' EQUICONSISTENT']. fold (MaximallyConsistentSet (AddHenkin (E.image embed_frm Gamma))) in SUBSET', IS_FILTER', COMPLETE', EQUICONSISTENT'.
-  pose proof (theorem_of_1_3_10 Gamma) as [? ? ? ? ? ?]. unnw.
+  pose proof (@theorem_of_1_3_10 L augmented_language_isEnumerable Gamma) as [? ? ? ? ? ?]; unnw.
   assert (claim : Gamma ⊭ Bot_frm).
-  { intros SAT. contradiction (SAT (restrict_structure (mkModel Gamma)) (ivar_interpret Gamma)).
-    - red. set (STRUCTURE := mkModel Gamma). set (env := ivar_interpret Gamma).
+  { intros SAT. contradiction (SAT (restrict_structure (trmModel Gamma)) (ivar_interpret Gamma)).
+    - red. set (STRUCTURE := trmModel Gamma). set (env := ivar_interpret Gamma).
       assert (MODEL : forall p : frm L, interpret_frm STRUCTURE env (embed_frm p) <-> interpret_frm (restrict_structure STRUCTURE) env p).
       { intros p. eapply restrict_structure_frm. }
-      ii. red. rewrite <- MODEL. unfold STRUCTURE, env. rewrite <- mkModel_isModel; trivial.
+      ii. red. rewrite <- MODEL. unfold STRUCTURE, env. rewrite <- trmModel_isModel; trivial.
       eapply SUBSET. rewrite in_Th_iff. eapply ByAssumption. done!.
     - simpl. intros t. unfold interpret_equation, ivar_interpret. simpl. eapply proves_reflexivity.
   }
