theories/Logic/HilbertFol2.v
@@ -1421,4 +1421,149 @@ Qed.
 
 End HENKIN.
 
+Section MODEL_EXISTENCE.
+
+#[local] Existing Instance V.vec_isSetoid.
+
+Context {L : language} {function_symbols_countable : isCountable L.(function_symbols)} {constant_symbols_countable : isCountable L.(constant_symbols)} {relation_symbols_countable : isCountable L.(relation_symbols)}.
+
+Notation L' := (augmented_language L Henkin_constants).
+
+#[local]
+Instance augmented_language_isEnumerable : isEnumerable (frm L') :=
+  @frm_isEnumerable L' function_symbols_countable (@sum_isCountable L.(constant_symbols) Henkin_constants constant_symbols_countable (isCountable_if_isEnumerable nat_isEnumerable)) relation_symbols_countable.
+
+Variable X : ensemble (frm L).
+
+Let Delta : ensemble (frm L') :=
+  MaximallyConsistentSet (AddHenkin (E.image embed_frm X)).
+
+Let D : Type :=
+  trm L'.
+
+Definition interpret_equation (lhs : D) (rhs : D) : Prop :=
+  Delta ⊢ Eqn_frm lhs rhs.
+
+#[global]
+Instance interpret_equation_Equivalence
+  : Equivalence interpret_equation.
+Proof with eauto.
+  unfold interpret_equation. split.
+  - intros x. eapply proves_reflexivity...
+  - intros x y EQ. eapply proves_symmetry...
+  - intros x y z EQ EQ'. eapply proves_transitivity...
+Qed.
+
+Lemma pairwise_equal_intro n vs1 vs2
+  (EQ : forall i : Fin.t n, interpret_equation (vs1 !! i) (vs2 !! i))
+  : pairwise_equal Delta (vec_to_trms vs1) (vec_to_trms vs2).
+Proof.
+  revert vs2 EQ. induction vs1 as [ | n v1 vs1 IH].
+  - introVNil; simpl; i. econs.
+  - introVCons v2 vs2; simpl; i. econs.
+    + eapply EQ with (i := FZ).
+    + eapply IH. intros i. eapply EQ with (i := FS i).
+Qed.
+
+Lemma pairwise_equal_symmetry n (vs1 : Vector.t (trm L') n) (vs2 : Vector.t (trm L') n)
+  (EQUAL : pairwise_equal Delta (vec_to_trms vs1) (vec_to_trms vs2))
+  : pairwise_equal Delta (vec_to_trms vs2) (vec_to_trms vs1).
+Proof.
+  revert vs2 EQUAL. induction vs1 as [ | n v1 vs1 IH].
+  - introVNil; simpl; i. econs.
+  - introVCons v2 vs2; simpl; intros [EQ EQUAL]. econs.
+    + eapply proves_symmetry; trivial.
+    + eapply IH; trivial.
+Qed.
+
+#[local, program]
+Instance trmModel : isStructureOf L' :=
+  { domain_of_discourse := D
+  ; equation_interpret := {| eqProp := interpret_equation; eqProp_Equivalence := interpret_equation_Equivalence |}
+  ; function_interpret f vs := Fun_trm f (vec_to_trms vs)
+  ; constant_interpret c := Con_trm c
+  ; relation_interpret R vs := Delta ⊢ Rel_frm R (vec_to_trms vs)
+  }.
+Next Obligation.
+  econs. exact (Var_trm 0).
+Qed.
+Next Obligation.
+  red. eapply proves_eqn_fun. eapply pairwise_equal_intro; trivial.
+Qed.
+Next Obligation.
+  split; intros INFERS.
+  - eapply for_Imp_E. eapply proves_eqn_rel. 2: exact INFERS. eapply pairwise_equal_intro; trivial.
+  - eapply for_Imp_E. eapply proves_eqn_rel. 2: exact INFERS. eapply pairwise_equal_symmetry; eapply pairwise_equal_intro; trivial.
+Qed.
+
+Definition ivar_interpret : ivar -> domain_of_discourse :=
+  Var_trm.
+
+Lemma interpret_trm_trmModel_ivar_interpret (t : trm L')
+  : interpret_trm trmModel ivar_interpret t = t
+with interpret_trms_trmModel_ivar_interpret n (ts : trms L' n)
+  : vec_to_trms (interpret_trms trmModel ivar_interpret ts) = ts.
+Proof.
+  - trm_ind t; simpl.
+    + reflexivity.
+    + rewrite interpret_trm_unfold. simpl. f_equal. eapply interpret_trms_trmModel_ivar_interpret.
+    + reflexivity.
+  - trms_ind ts.
+    + reflexivity.
+    + rewrite interpret_trms_unfold. simpl. f_equal.
+      * eapply interpret_trm_trmModel_ivar_interpret.
+      * eapply IH.
+Qed.
+
+Hypothesis CONSISTENT : X ⊬ Bot_frm.
+
+Theorem trmModel_isModel (p : frm L')
+  : p \in Delta <-> interpret_frm trmModel ivar_interpret p.
+Proof with eauto with *.
+  exploit (@theorem_of_1_2_14 (frm L') (@formula_isSetoid L') LindenbaumBooleanAlgebra (Th (AddHenkin (E.image embed_frm X)))).
+  { eapply lemma1_of_1_3_8. }
+  intros [SUBSET' IS_FILTER' COMPLETE' EQUICONSISTENT']. fold (MaximallyConsistentSet (AddHenkin (E.image embed_frm X))) in SUBSET', IS_FILTER', COMPLETE', EQUICONSISTENT'.
+  fold Delta in SUBSET', IS_FILTER', COMPLETE', EQUICONSISTENT'.
+  pose proof (theorem_of_1_3_10 X) as [? ? ? ? ? ?]. fold Delta in SUBSET, EQUICONSISTENT, CLOSED_infers, META_DN, IMPLICATION_FAITHFUL, FORALL_FAITHFUL. unnw.
+  assert (CONSISTENT' : Delta ⊬ Bot_frm).
+  { intros INCONSISTENT.
+    assert (claim1 : ~ inconsistent' Delta).
+    { red in EQUICONSISTENT'. rewrite <- EQUICONSISTENT'. rewrite <- cl_eq_Th. rewrite <- inconsistent_okay. rewrite <- AddHenkin_equiconsistent.
+      - rewrite <- similar_equiconsistent with (Gamma := X).
+        + rewrite inconsistent_iff; trivial.
+        + rewrite <- embed_frms_spec. reflexivity.
+      - ii. rewrite E.in_image_iff in H. destruct H as [q [-> IN]]. eapply embed_frm_HC_free.
+    }
+    contradiction claim1. rewrite <- inconsistent_iff in INCONSISTENT.
+    rewrite inconsistent_okay in INCONSISTENT. eapply inconsistent_compatWith_isSubsetOf... eapply fact5_of_1_2_8...
+  }
+  rewrite CLOSED_infers. pattern p. revert p. eapply @frm_depth_lt_ind. intros [R ts | t1 t2 | p1 | p1 p2 | y p1]; simpl; i.
+  - rewrite interpret_trms_trmModel_ivar_interpret. reflexivity.
+  - do 2 rewrite interpret_trm_trmModel_ivar_interpret. reflexivity.
+  - rewrite <- IH with (p' := p1). 2: lia. split.
+    + intros INFERS1 INFERS2. contradiction CONSISTENT'.
+      eapply ContradictionI with (A := p1); trivial.
+    + intros NO. rewrite <- CLOSED_infers. eapply META_DN. intros YES. rewrite CLOSED_infers.
+      contradiction NO. rewrite CLOSED_infers in YES. eapply NegationE. eapply ContradictionI with (A := Neg_frm p1).
+      * eapply ByAssumption; done!.
+      * eapply extend_infers with (Gamma := Delta); done!.
+  - rewrite <- IH with (p' := p1). 2: lia. rewrite <- IH with (p' := p2). 2: lia. split.
+    + intros INFERS1 INFERS2. eapply ImplicationE with (A := p1); trivial.
+    + intros INFERS. rewrite <- CLOSED_infers. eapply IMPLICATION_FAITHFUL. do 2 rewrite CLOSED_infers; trivial.
+  - unfold D. split.
+    + intros INFERS t. rename y into x. set (s := one_subst x t).
+      assert (IFF : interpret_frm trmModel ivar_interpret (subst_frm s p1) <-> interpret_frm trmModel (upd_env x t ivar_interpret) p1).
+      { rewrite <- substitution_lemma_frm. eapply interpret_frm_ext. ii. unfold compose, upd_env, s, one_subst, cons_subst, nil_subst.
+        destruct (eq_dec z x) as [EQ1 | NE1]; trivial. eapply interpret_trm_trmModel_ivar_interpret.
+      }
+      rewrite <- IFF. rewrite <- IH with (p' := subst_frm s p1). 2: rewrite subst_preserves_rank; lia.
+      unfold s. eapply for_All_E; trivial.
+    + intros INTERPRET. rewrite <- CLOSED_infers. eapply FORALL_FAITHFUL.
+      intros t. eapply CLOSED_infers. rewrite -> IH with (p' := subst_frm (one_subst y t) p1). 2: rewrite subst_preserves_rank; lia.
+      rewrite <- substitution_lemma_frm. eapply interpret_frm_ext with (env' := upd_env y (interpret_trm trmModel ivar_interpret t) ivar_interpret). ii. unfold compose, upd_env, one_subst, cons_subst, nil_subst.
+      destruct (eq_dec z y) as [EQ1 | NE1]; trivial. eapply INTERPRET.
+Qed.
+
+End MODEL_EXISTENCE.
+
 End FolHilbert.
