theories/Math/ConstructiveOrdinal.v
@@ -1,3 +1,35 @@
 Require Import PnV.Prelude.Prelude.
 Require Import PnV.Math.OrderTheory.
 Require Import PnV.Data.Aczel.
+
+Module TypeTheoreticOrdinals.
+
+Definition ord : Type@{Set_V} :=
+  Tree.
+
+#[global]
+Instance ord_isWellPoset : isWellPoset ord :=
+  { wltProp := rLt
+  ; wltProp_Transitive := rLt_StrictOrder.(StrictOrder_Transitive)
+  ; wltProp_well_founded := rLt_wf 
+  }.
+
+Section TRANSFINITE.
+
+Context {D : Type@{Set_V}} (suc : D -> D) (lim : forall A : Type@{Set_u}, (A -> D) -> D).
+
+Fixpoint tf_rec (o : ord) {struct o} : D :=
+  match o with
+  | mkNode cs ts => lim cs (fun c => suc (tf_rec (ts c)))
+  end.
+
+End TRANSFINITE.
+
+Section HARTOGS.
+
+Definition Hartogs (D : Type@{Set_u}) : ord :=
+  mkNode { R : D -> D -> Prop | well_founded R } (fun RWF => @fromWf D (proj1_sig RWF) (proj2_sig RWF)).
+
+End HARTOGS.
+
+End TypeTheoreticOrdinals.
